Use new order for safe conversion

safechecker/theories/PCUICSafeConversion.v
@@ -266,11 +266,10 @@ Section Conversion.
 
   (* Definition weq_term_pos {Γ} (u v : wterm Γ) (e : weqt u v) (p : pos u) *)
 
-  (* Alternative definition of R_aux, to replace it eventually *)
-  Equations R_aux' (Γ : context) :
+  Equations R_aux (Γ : context) :
     (∑ t : term, pos t × (∑ w : wterm Γ, pos (` w) × state)) ->
     (∑ t : term, pos t × (∑ w : wterm Γ, pos (` w) × state)) -> Prop :=
-    R_aux' Γ :=
+    R_aux Γ :=
       t ⊨ eqt \ cored' Σ Γ by _ ⨷
       @posR t ⊗
       w ⊨ weqt \ wcored Γ by _ ⨷
@@ -291,30 +290,17 @@ Section Conversion.
     eapply eq_term_valid_pos. all: eauto.
   Defined.
 
-  (* Transparent R_aux'. *)
-
-  (* Several things:
-     - We need to show valid_pos is preserved by eq_term
-     - We need to use eq_term for cored' and not just upto_names
-     - Which of eq_term/leq_term? We want to account for both...
-
-     => Probably just eq_term
-     => This might only be interesting in cases like tCase where we
-     compare stuff with nl_eq,
-     for stacks we might want to keep both terms in the end
-     (no more zipc_replace!) and instead carry the information
-     that they are eq or leq.
-  *)
+  (* Transparent R_aux. *)
 
   Derive Signature for Subterm.lexprod.
 
-  Lemma R_aux'_Acc :
+  Lemma R_aux_Acc :
     forall Γ t p w q s,
       wellformed Σ Γ t ->
-      Acc (R_aux' Γ) (t ; (p, (w ; (q, s)))).
+      Acc (R_aux Γ) (t ; (p, (w ; (q, s)))).
   Proof.
     intros Γ t p w q s ht.
-    rewrite R_aux'_equation_1.
+    rewrite R_aux_equation_1.
     unshelve eapply dlexmod_Acc.
     - intros x y [e]. constructor. eapply eq_term_sym. assumption.
     - intros x y z [e1] [e2]. constructor. eapply eq_term_trans. all: eauto.
@@ -332,15 +318,15 @@ Section Conversion.
           -- constructor. assumption.
           -- constructor. eapply eq_term_trans. all: eauto.
         * intros x. exists (sq (eq_term_refl _ _)). intros [[q'' h] ?].
-          unfold R_aux'_obligations_obligation_2.
+          unfold R_aux_obligations_obligation_2.
           simpl. f_equal. f_equal.
           eapply uip.
         * intros x x' [[q'' h] ?] [e].
-          unfold R_aux'_obligations_obligation_2.
+          unfold R_aux_obligations_obligation_2.
           simpl. f_equal. f_equal.
           eapply uip.
         * intros x y z e1 e2 [[q'' h] ?].
-          unfold R_aux'_obligations_obligation_2.
+          unfold R_aux_obligations_obligation_2.
           simpl. f_equal. f_equal.
           eapply uip.
         * intros [t1 ht1] [t2 ht2] [e] [[q1 hq1] s1] [[q2 hq2] s2] h.
@@ -358,15 +344,15 @@ Section Conversion.
       + constructor. assumption.
       + constructor. eapply eq_term_trans. all: eauto.
     - intros x. exists (sq (eq_term_refl _ _)). intros [[q' h] [? [? ?]]].
-      unfold R_aux'_obligations_obligation_1.
+      unfold R_aux_obligations_obligation_1.
       simpl. f_equal. f_equal.
       eapply uip.
     - intros x x' [[q' h] [? [? ?]]] [e].
-      unfold R_aux'_obligations_obligation_1.
+      unfold R_aux_obligations_obligation_1.
       simpl. f_equal. f_equal.
       eapply uip.
     - intros x y z e1 e2 [[q' h] [? [? ?]]].
-      unfold R_aux'_obligations_obligation_1.
+      unfold R_aux_obligations_obligation_1.
       simpl. f_equal. f_equal.
       eapply uip.
     - intros x x' [e]
@@ -392,9 +378,6 @@ Section Conversion.
     - eapply normalisation_upto. all: assumption.
   Qed.
 
-  Definition R_aux Γ :=
-    t ⊩ cored' Σ Γ ⨶ @posR t ⊗ w ⊩ wcored Γ ⨶ @posR (` w) ⊗ stateR.
-
   Notation pzt u := (zipc (tm u) (stk1 u)) (only parsing).
   Notation pps1 u := (stack_pos (tm u) (stk1 u)) (only parsing).
   Notation pwt u := (exist _ (wth u)) (only parsing).
@@ -403,29 +386,8 @@ Section Conversion.
   Notation obpack u :=
     (pzt u ; (pps1 u, (pwt u ; (pps2 u, st u)))) (only parsing).
 
-  Definition R_nl Γ (u v : pack Γ) :=
-    R_aux Γ (obpack u) (obpack v).
-
   Definition R Γ (u v : pack Γ) :=
-    R_nl (nlctx Γ) (nl_pack u) (nl_pack v).
-
-  Lemma R_aux_Acc :
-    forall Γ t p w q s,
-      wellformed Σ Γ t ->
-      Acc (R_aux Γ) (t ; (p, (w ; (q, s)))).
-  Proof.
-    intros Γ t p w q s ht.
-    eapply dlexprod_Acc.
-    - intro u. eapply Subterm.wf_lexprod.
-      + intro. eapply posR_Acc.
-      + intros [w' q']. eapply dlexprod_Acc.
-        * intros [t' h']. eapply Subterm.wf_lexprod.
-          -- intro. eapply posR_Acc.
-          -- intro. eapply stateR_Acc.
-        * eapply wcored_wf.
-    - destruct hΣ as [hΣ'].
-      eapply normalisation_upto. all: assumption.
-  Qed.
+    R_aux Γ (obpack u) (obpack v).
 
   Lemma R_Acc :
     forall Γ u,
@@ -433,12 +395,8 @@ Section Conversion.
       Acc (R Γ) u.
   Proof.
     intros Γ u h.
-    eapply Acc_fun with (f := fun x => obpack (nl_pack x)).
-    apply R_aux_Acc.
-    rewrite <- nl_zipc.
-    eapply wellformed_nlctx; tas.
-    eapply wellformed_alpha ; try eassumption.
-    eapply eq_term_upto_univ_tm_nl. all: auto.
+    eapply Acc_fun with (f := fun x => obpack x).
+    apply R_aux_Acc. assumption.
   Qed.
 
   Lemma R_cored :
@@ -447,100 +405,110 @@ Section Conversion.
       R Γ p1 p2.
   Proof.
     intros Γ p1 p2 h.
-    left. rewrite <- 2!nl_zipc.
-    eapply cored_cored'_nl. assumption.
+    left. eapply cored_cored'. assumption.
   Qed.
 
   Lemma R_aux_positionR :
     forall Γ t1 t2 (p1 : pos t1) (p2 : pos t2) s1 s2,
-      t1 = t2 ->
+      eq_term Σ t1 t2 ->
       positionR (` p1) (` p2) ->
       R_aux Γ (t1 ; (p1, s1)) (t2 ; (p2, s2)).
   Proof.
-    intros Γ t1 t2 p1 p2 s1 s2 e h.
-    subst. right. left. assumption.
+    intros Γ t1 t2 p1 p2 [? [? ?]] s2 e h.
+    unshelve eright.
+    - constructor. assumption.
+    - left. unfold posR. simpl. assumption.
   Qed.
 
   Lemma R_positionR :
     forall Γ p1 p2,
-      nl (pzt p1) = nl (pzt p2) ->
+      eq_term Σ (pzt p1) (pzt p2) ->
       positionR (` (pps1 p1)) (` (pps1 p2)) ->
       R Γ p1 p2.
   Proof.
     intros Γ [s1 t1 π1 ρ1 t1' h1] [s2 t2 π2 ρ2 t2' h2] e h. simpl in *.
     eapply R_aux_positionR ; simpl.
-    - rewrite <- 2!nl_zipc. assumption.
-    - rewrite 2!stack_position_nlstack.
-      assumption.
+    - assumption.
+    - assumption.
   Qed.
 
   Lemma R_aux_cored2 :
     forall Γ t1 t2 (p1 : pos t1) (p2 : pos t2) w1 w2 q1 q2 s1 s2,
-      t1 = t2 ->
+      eq_term Σ t1 t2 ->
       ` p1 = ` p2 ->
       cored' Σ Γ (` w1) (` w2) ->
       R_aux Γ (t1 ; (p1, (w1 ; (q1, s1)))) (t2 ; (p2, (w2 ; (q2, s2)))).
   Proof.
     intros Γ t1 t2 [p1 hp1] [p2 hp2] [t1' h1'] [t2' h2'] q1 q2 s1 s2 e1 e2 h.
     cbn in e2. cbn in h. subst.
-    pose proof (uip hp1 hp2). subst.
-    right. right. left. assumption.
+    unshelve eright.
+    - constructor. assumption.
+    - unfold R_aux_obligations_obligation_1. simpl.
+      match goal with
+      | |- context [ exist p2 ?hp1 ] =>
+        assert (e : hp1 = hp2) by eapply uip
+      end.
+      rewrite e.
+      right.
+      left. assumption.
   Qed.
 
   Lemma R_cored2 :
     forall Γ p1 p2,
-      nl (pzt p1) = nl (pzt p2) ->
+      eq_term Σ (pzt p1) (pzt p2) ->
       ` (pps1 p1) = ` (pps1 p2) ->
       cored Σ Γ (` (pwt p1)) (` (pwt p2)) ->
       R Γ p1 p2.
   Proof.
     intros Γ [s1 t1 π1 ρ1 t1' h1] [s2 t2 π2 ρ2 t2' h2] e1 e2 h. simpl in *.
-    eapply R_aux_cored2 ; simpl.
-    - rewrite <- 2!nl_zipc. assumption.
-    - rewrite 2!stack_position_nlstack. assumption.
-    - destruct s1, s2 ; simpl.
-      all: rewrite <- 2!nl_zipc.
-      all: eapply cored_cored'_nl ; auto.
+    eapply R_aux_cored2. all: simpl. all: auto.
+    destruct s1, s2.
+    all: eapply cored_cored'.
+    all: assumption.
   Qed.
 
   Lemma R_aux_positionR2 :
     forall Γ t1 t2 (p1 : pos t1) (p2 : pos t2) w1 w2 q1 q2 s1 s2,
-      t1 = t2 ->
+      eq_term Σ t1 t2 ->
       ` p1 = ` p2 ->
-      ` w1 = ` w2 ->
+      eq_term Σ (` w1) (` w2) ->
       positionR (` q1) (` q2) ->
       R_aux Γ (t1 ; (p1, (w1 ; (q1, s1)))) (t2 ; (p2, (w2 ; (q2, s2)))).
   Proof.
     intros Γ t1 t2 [p1 hp1] [p2 hp2] [t1' h1'] [t2' h2'] q1 q2 s1 s2 e1 e2 e3 h.
     cbn in e2. cbn in e3. subst.
-    pose proof (uip hp1 hp2). subst.
-    pose proof (wellformed_irr h1' h2'). subst.
-    right. right. right. left. assumption.
+    unshelve eright.
+    - constructor. assumption.
+    - unfold R_aux_obligations_obligation_1. simpl.
+      match goal with
+      | |- context [ exist p2 ?hp1 ] =>
+        assert (e : hp1 = hp2) by eapply uip
+      end.
+      rewrite e.
+      right.
+      unshelve eright.
+      + constructor. assumption.
+      + left. unfold posR. simpl. assumption.
   Qed.
 
   Lemma R_positionR2 :
     forall Γ p1 p2,
-      nl (pzt p1) = nl (pzt p2) ->
+      eq_term Σ (pzt p1) (pzt p2) ->
       ` (pps1 p1) = ` (pps1 p2) ->
-      nl (` (pwt p1)) = nl (` (pwt p2)) ->
+      eq_term Σ (` (pwt p1)) (` (pwt p2)) ->
       positionR (` (pps2 p1)) (` (pps2 p2)) ->
       R Γ p1 p2.
   Proof.
     intros Γ [s1 t1 π1 ρ1 t1' h1] [s2 t2 π2 ρ2 t2' h2] e1 e2 e3 h.
     simpl in *.
-    eapply R_aux_positionR2 ; simpl.
-    - rewrite <- 2!nl_zipc. assumption.
-    - rewrite 2!stack_position_nlstack. assumption.
-    - destruct s1, s2 ; simpl.
-      all: rewrite <- 2!nl_zipc. all: assumption.
-    - rewrite 2!stack_position_nlstack. assumption.
+    eapply R_aux_positionR2. all: simpl. all: auto.
   Qed.
 
   Lemma R_aux_stateR :
     forall Γ t1 t2 (p1 : pos t1) (p2 : pos t2) w1 w2 q1 q2 s1 s2 ,
-      t1 = t2 ->
+      eq_term Σ t1 t2 ->
       ` p1 = ` p2 ->
-      ` w1 = ` w2 ->
+      eq_term Σ (` w1) (` w2) ->
       ` q1 = ` q2 ->
       stateR s1 s2 ->
       R_aux Γ (t1 ; (p1, (w1 ; (q1, s1)))) (t2 ; (p2, (w2 ; (q2, s2)))).
@@ -548,30 +516,182 @@ Section Conversion.
     intros Γ t1 t2 [p1 hp1] [p2 hp2] [t1' h1'] [t2' h2'] [q1 hq1] [q2 hq2] s1 s2
            e1 e2 e3 e4 h.
     cbn in e2. cbn in e3. cbn in e4. subst.
-    pose proof (uip hp1 hp2). subst.
-    pose proof (wellformed_irr h1' h2'). subst.
-    pose proof (uip hq1 hq2). subst.
-    right. right. right. right. assumption.
+    unshelve eright.
+    - constructor. assumption.
+    - unfold R_aux_obligations_obligation_1. simpl.
+      match goal with
+      | |- context [ exist p2 ?hp1 ] =>
+        assert (e : hp1 = hp2) by eapply uip
+      end.
+      rewrite e.
+      right.
+      unshelve eright.
+      + constructor. assumption.
+      + unfold R_aux_obligations_obligation_2. simpl.
+        match goal with
+        | |- context [ exist q2 ?hq1 ] =>
+          assert (e' : hq1 = hq2) by eapply uip
+        end.
+        rewrite e'.
+        right. assumption.
   Qed.
 
   Lemma R_stateR :
     forall Γ p1 p2,
-      nl (pzt p1) = nl (pzt p2) ->
+      eq_term Σ (pzt p1) (pzt p2) ->
       ` (pps1 p1) = ` (pps1 p2) ->
-      nl (` (pwt p1)) = nl (` (pwt p2)) ->
+      eq_term Σ (` (pwt p1)) (` (pwt p2)) ->
       ` (pps2 p1) = ` (pps2 p2) ->
       stateR (st p1) (st p2) ->
       R Γ p1 p2.
   Proof.
     intros Γ [s1 t1 π1 ρ1 t1' h1] [s2 t2 π2 ρ2 t2' h2] e1 e2 e3 e4 h.
     simpl in *.
-    eapply R_aux_stateR ; simpl.
-    - rewrite <- 2!nl_zipc. assumption.
-    - rewrite 2!stack_position_nlstack. assumption.
-    - destruct s1, s2 ; simpl.
-      all: rewrite <- 2!nl_zipc. all: assumption.
-    - rewrite 2!stack_position_nlstack. assumption.
-    - induction h ; constructor.
+    eapply R_aux_stateR. all: simpl. all: auto.
+  Qed.
+
+  (* TODO MOVE *)
+  Lemma eqb_term_upto_univ_refl :
+    forall (eqb leqb : universe -> universe -> bool) t,
+      (forall u, eqb u u) ->
+      (forall u, leqb u u) ->
+      eqb_term_upto_univ eqb leqb t t.
+  Admitted.
+
+  Definition leqb_term :=
+    eqb_term_upto_univ (try_eqb_universe G) (try_leqb_universe G).
+
+  Definition eqb_term :=
+    eqb_term_upto_univ (try_eqb_universe G) (try_eqb_universe G).
+
+  Lemma leqb_term_spec t u :
+    leqb_term t u ->
+    leq_term (global_ext_constraints Σ) t u.
+  Proof.
+    pose proof hΣ'.
+    apply eqb_term_upto_univ_impl.
+    intros u1 u2; eapply (try_eqb_universe_spec G (global_ext_uctx Σ)); tas.
+    now eapply wf_ext_global_uctx_invariants.
+    now eapply global_ext_uctx_consistent.
+    intros u1 u2; eapply (try_leqb_universe_spec G (global_ext_uctx Σ)); tas.
+    now eapply wf_ext_global_uctx_invariants.
+    now eapply global_ext_uctx_consistent.
+  Qed.
+
+  Lemma eqb_term_spec t u :
+    eqb_term t u ->
+    eq_term (global_ext_constraints Σ) t u.
+  Proof.
+    pose proof hΣ'.
+    apply eqb_term_upto_univ_impl.
+    intros u1 u2; eapply (try_eqb_universe_spec G (global_ext_uctx Σ)); tas.
+    now eapply wf_ext_global_uctx_invariants.
+    now eapply global_ext_uctx_consistent.
+    intros u1 u2; eapply (try_eqb_universe_spec G (global_ext_uctx Σ)); tas.
+    now eapply wf_ext_global_uctx_invariants.
+    now eapply global_ext_uctx_consistent.
+  Qed.
+
+  Lemma leqb_term_refl :
+    forall t, leqb_term t t.
+  Proof.
+    intro t. eapply eqb_term_upto_univ_refl.
+  Admitted.
+
+  Lemma eqb_term_refl :
+    forall t, eqb_term t t.
+  Admitted.
+
+  Fixpoint eqb_ctx (Γ Δ : context) : bool :=
+    match Γ, Δ with
+    | [], [] => true
+    | {| decl_name := na1 ; decl_body := None ; decl_type := t1 |} :: Γ,
+      {| decl_name := na2 ; decl_body := None ; decl_type := t2 |} :: Δ =>
+      eqb_term t1 t2 && eqb_ctx Γ Δ
+    | {| decl_name := na1 ; decl_body := Some b1 ; decl_type := t1 |} :: Γ,
+      {| decl_name := na2 ; decl_body := Some b2 ; decl_type := t2 |} :: Δ =>
+      eqb_term b1 b2 && eqb_term t1 t2 && eqb_ctx Γ Δ
+    | _, _ => false
+    end.
+
+  Lemma eqb_ctx_spec :
+    forall Γ Δ,
+      eqb_ctx Γ Δ ->
+      eq_context_upto (eq_universe (global_ext_constraints Σ)) Γ Δ.
+  Proof.
+    intros Γ Δ h.
+    induction Γ as [| [na [b|] A] Γ ih ] in Δ, h |- *.
+    all: destruct Δ as [| [na' [b'|] A'] Δ].
+    all: try discriminate.
+    - constructor.
+    - simpl in h. apply andP in h as [h h3]. apply andP in h as [h1 h2].
+      constructor.
+      + eapply eqb_term_spec. assumption.
+      + eapply eqb_term_spec. assumption.
+      + eapply ih. assumption.
+    - simpl in h. apply andP in h as [h1 h2].
+      constructor.
+      + eapply eqb_term_spec. assumption.
+      + eapply ih. assumption.
+  Qed.
+
+  Definition eqb_term_stack t1 π1 t2 π2 :=
+    eqb_ctx (stack_context π1) (stack_context π2) &&
+    eqb_term (zipp t1 π1) (zipp t2 π2).
+
+  Lemma eqb_term_stack_spec :
+    forall Γ t1 π1 t2 π2,
+      eqb_term_stack t1 π1 t2 π2 ->
+      eq_context_upto (eq_universe (global_ext_constraints Σ))
+                      (Γ ,,, stack_context π1)
+                      (Γ ,,, stack_context π2) ×
+      eq_term (global_ext_constraints Σ) (zipp t1 π1) (zipp t2 π2).
+  Proof.
+    intros Γ t1 π1 t2 π2 h.
+    apply andP in h as [h1 h2].
+    split.
+    - eapply eq_context_upto_cat.
+      + eapply eq_context_upto_refl. intro. apply eq_universe_refl.
+      + eapply eqb_ctx_spec. assumption.
+    - eapply eqb_term_spec. assumption.
+  Qed.
+
+  Definition leqb_term_stack t1 π1 t2 π2 :=
+    eqb_ctx (stack_context π1) (stack_context π2) &&
+    leqb_term (zipp t1 π1) (zipp t2 π2).
+
+  Definition eqb_termp leq u v :=
+    match leq with
+    | Conv => eqb_term u v
+    | Cumul => leqb_term u v
+    end.
+
+  Lemma eqb_termp_spec :
+    forall leq u v Γ,
+      eqb_termp leq u v ->
+      conv leq Σ Γ u v.
+  Proof.
+    intros leq u v Γ e.
+    destruct leq.
+    - simpl. constructor. constructor. eapply eqb_term_spec. assumption.
+    - simpl. constructor. constructor. eapply leqb_term_spec. assumption.
+  Qed.
+
+  Lemma leqb_term_stack_spec :
+    forall Γ t1 π1 t2 π2,
+      leqb_term_stack t1 π1 t2 π2 ->
+      eq_context_upto (eq_universe (global_ext_constraints Σ))
+                      (Γ ,,, stack_context π1)
+                      (Γ ,,, stack_context π2) ×
+      leq_term (global_ext_constraints Σ) (zipp t1 π1) (zipp t2 π2).
+  Proof.
+    intros Γ t1 π1 t2 π2 h.
+    apply andP in h as [h1 h2].
+    split.
+    - eapply eq_context_upto_cat.
+      + eapply eq_context_upto_refl. intro. apply eq_universe_refl.
+      + eapply eqb_ctx_spec. assumption.
+    - eapply leqb_term_spec. assumption.
   Qed.
 
   Lemma zwts :
@@ -586,11 +706,6 @@ Section Conversion.
   Notation conv_stack_ctx Γ π1 π2 :=
     (∥ conv_context Σ (Γ ,,, stack_context π1) (Γ ,,, stack_context π2) ∥).
 
-  (* Notation conv_term leq Γ t π t' π' :=
-    (conv_stack_ctx Γ π π' /\
-     conv leq Σ (Γ ,,, stack_context π) (zipp t π) (zipp t' π'))
-      (only parsing). *)
-
   Notation conv_term leq Γ t π t' π' :=
     (conv leq Σ (Γ ,,, stack_context π) (zipp t π) (zipp t' π'))
       (only parsing).
@@ -598,10 +713,6 @@ Section Conversion.
   Notation alt_conv_term Γ t π π' :=
     (∥ Σ ;;; Γ ,,, stack_context π |- zipp t π == zipp t π' ∥)
       (only parsing).
-
-  (* Notation alt_conv_term Γ t π π' :=
-    (conv_stack_ctx Γ π π' /\ alt_conv_term' Γ t π π')
-      (only parsing). *)
 
   (* Definition Ret s Γ t π π' := *)
   (*   match s with *)
@@ -1437,13 +1548,12 @@ Section Conversion.
       | @exist false _ := no
       } ;
 
-    (* TODO Replace nleq_term here by eq_term (x3) *)
     | prog_view_Case ind par p c brs ind' par' p' c' brs'
-      with inspect (nleq_term (tCase (ind, par) p c brs) (tCase (ind', par') p' c' brs')) := {
+      with inspect (eqb_term (tCase (ind, par) p c brs) (tCase (ind', par') p' c' brs')) := {
       | @exist true eq1 := isconv_args (tCase (ind, par) p c brs) π1 π2 aux ;
       | @exist false _ with inspect (reduce_term RedFlags.default Σ hΣ (Γ ,,, stack_context π1) c _) := {
         | @exist cred eq1 with inspect (reduce_term RedFlags.default Σ hΣ (Γ ,,, stack_context π2) c' _) := {
-           | @exist cred' eq2 with inspect (nleq_term cred c && nleq_term cred' c') := {
+           | @exist cred' eq2 with inspect (eqb_term cred c && eqb_term cred' c') := {
               | @exist true eq3 := no ;
               | @exist false eq3 :=
                 isconv_red leq (tCase (ind, par) p cred brs) π1
@@ -1453,15 +1563,13 @@ Section Conversion.
         }
       } ;
 
-    (* TODO Replace nleq_term here by eq_term *)
-    | prog_view_Proj p c p' c' with inspect (nleq_term (tProj p c) (tProj p' c')) := {
+    | prog_view_Proj p c p' c' with inspect (eqb_term (tProj p c) (tProj p' c')) := {
       | @exist true eq1 := isconv_args (tProj p c) π1 π2 aux ;
       | @exist false _ := no
       } ;
 
-    (* TODO Replace nleq_term here by eq_term *)
     | prog_view_Fix mfix idx mfix' idx'
-      with inspect (nleq_term (tFix mfix idx) (tFix mfix' idx')) := {
+      with inspect (eqb_term (tFix mfix idx) (tFix mfix' idx')) := {
       | @exist true eq1 := isconv_args (tFix mfix idx) π1 π2 aux ;
       | @exist false _ with inspect (unfold_one_fix Γ mfix idx π1 _) := {
         | @exist (Some (fn, θ)) eq1
@@ -1486,9 +1594,8 @@ Section Conversion.
         }
       } ;
 
-    (* TODO Replace nleq_term here by eq_term *)
     | prog_view_CoFix mfix idx mfix' idx'
-      with inspect (nleq_term (tCoFix mfix idx) (tCoFix mfix' idx')) := {
+      with inspect (eqb_term (tCoFix mfix idx) (tCoFix mfix' idx')) := {
       | @exist true eq1 := isconv_args (tCoFix mfix idx) π1 π2 aux ;
       | @exist false _ := no
       } ;
@@ -1639,23 +1746,23 @@ Section Conversion.
 
   (* tCase *)
   Next Obligation.
-    symmetry in eq1.
+    (* TODO NEED wellformed upto eq_term *)
+    (* symmetry in eq1.
     eapply wellformed_alpha ; [ assumption .. | exact h2 |].
     eapply eq_term_upto_univ_sym. all: auto.
     eapply eq_term_upto_univ_zipc. all: auto.
     eapply elimT.
     - eapply reflect_upto_names.
     - assumption.
-  Qed.
+  Qed. *)
+  Admitted.
   Next Obligation.
     unshelve eapply R_stateR.
-    all: try reflexivity.
-    - simpl.
-      symmetry in eq1.
-      eapply ssrbool.elimT.
-      + eapply reflect_nleq_term.
-      + eapply nleq_term_zipc. assumption.
-    - simpl. constructor.
+    all: try reflexivity. all: simpl.
+    - symmetry in eq1.
+      apply eqb_term_spec in eq1.
+      apply eq_term_zipc. assumption.
+    - constructor.
   Qed.
   Next Obligation.
     destruct hΣ as [wΣ].
@@ -1665,11 +1772,8 @@ Section Conversion.
     eapply conv_alt_trans ; try eassumption.
     eapply conv_zipp.
     constructor.
-    symmetry in eq1.
-    eapply upto_names_impl_eq_term.
-    eapply elimT.
-    - eapply reflect_upto_names.
-    - assumption.
+    eapply eqb_term_spec.
+    eauto.
   Qed.
   Next Obligation.
     destruct hΣ as [wΣ].
@@ -1734,16 +1838,9 @@ Section Conversion.
         rewrite e in eq3.
         rewrite e' in eq3.
         cbn in eq3. symmetry in eq3.
-        assert (bot : eqb_term_upto_univ eqb eqb c c && eqb_term_upto_univ eqb eqb c' c').
-        { apply andb_and. split.
-          - eapply introT.
-            + eapply reflect_upto_names.
-            + eapply eq_term_upto_univ_refl. all: intro ; reflexivity.
-          - eapply introT.
-            + eapply reflect_upto_names.
-            + eapply eq_term_upto_univ_refl. all: intro ; reflexivity.
-        }
-        rewrite bot in eq3. discriminate.
+        apply andb_false_elim in eq3 as [bot | bot].
+        all: rewrite eqb_term_refl in bot.
+        all: discriminate.
       + dependent destruction hr.
         * unshelve eapply R_cored2.
           all: try reflexivity.
@@ -1755,16 +1852,9 @@ Section Conversion.
           rewrite e in eq3.
           rewrite <- H2 in eq3.
           cbn in eq3. symmetry in eq3.
-          assert (bot : eqb_term_upto_univ eqb eqb c c && eqb_term_upto_univ eqb eqb c' c').
-          { apply andb_and. split.
-            - eapply introT.
-              + eapply reflect_upto_names.
-              + eapply eq_term_upto_univ_refl. all: intro ; reflexivity.
-            - eapply introT.
-              + eapply reflect_upto_names.
-              + eapply eq_term_upto_univ_refl. all: intro ; reflexivity.
-          }
-          rewrite bot in eq3. discriminate.
+          apply andb_false_elim in eq3 as [bot | bot].
+          all: rewrite eqb_term_refl in bot.
+          all: discriminate.
     - dependent destruction hr.
       + eapply R_cored. simpl.
         eapply cored_zipc. eapply cored_case. assumption.
@@ -1778,16 +1868,9 @@ Section Conversion.
           rewrite e' in eq3.
           rewrite <- H2 in eq3.
           cbn in eq3. symmetry in eq3.
-          assert (bot : eqb_term_upto_univ eqb eqb c c && eqb_term_upto_univ eqb eqb c' c').
-          { apply andb_and. split.
-            - eapply introT.
-              + eapply reflect_upto_names.
-              + eapply eq_term_upto_univ_refl. all: intro ; reflexivity.
-            - eapply introT.
-              + eapply reflect_upto_names.
-              + eapply eq_term_upto_univ_refl. all: intro ; reflexivity.
-          }
-          rewrite bot in eq3. discriminate.
+          apply andb_false_elim in eq3 as [bot | bot].
+          all: rewrite eqb_term_refl in bot.
+          all: discriminate.
         * dependent destruction hr.
           -- unshelve eapply R_cored2.
              all: try reflexivity.
@@ -1802,16 +1885,9 @@ Section Conversion.
              rewrite <- H4 in eq3.
              rewrite <- H5 in eq3.
              cbn in eq3. symmetry in eq3.
-             assert (bot : eqb_term_upto_univ eqb eqb c c && eqb_term_upto_univ eqb eqb c' c').
-             { apply andb_and. split.
-               - eapply introT.
-                 + eapply reflect_upto_names.
-                 + eapply eq_term_upto_univ_refl. all: intro ; reflexivity.
-               - eapply introT.
-                 + eapply reflect_upto_names.
-                 + eapply eq_term_upto_univ_refl. all: intro ; reflexivity.
-             }
-             rewrite bot in eq3. discriminate.
+             apply andb_false_elim in eq3 as [bot | bot].
+             all: rewrite eqb_term_refl in bot.
+             all: discriminate.
   Qed.
   Next Obligation.
     destruct hΣ as [wΣ].
@@ -1850,7 +1926,8 @@ Section Conversion.
 
   (* tProj *)
   Next Obligation.
-    destruct hΣ as [wΣ].
+    (* TODO NEED *)
+    (* destruct hΣ as [wΣ].
     eapply wellformed_alpha ; try assumption.
     - exact h2.
     - apply eq_term_upto_univ_sym ; auto.
@@ -1858,16 +1935,15 @@ Section Conversion.
       eapply elimT.
       + eapply reflect_upto_names.
       + symmetry. assumption.
-  Qed.
+  Qed. *)
+  Admitted.
   Next Obligation.
     unshelve eapply R_stateR.
     all: try reflexivity.
-    - simpl.
-      eapply ssrbool.elimT.
-      + eapply reflect_nleq_term.
-      + eapply nleq_term_zipc.
-        symmetry. assumption.
-    - simpl. constructor.
+    all: simpl.
+    - eapply eq_term_zipc.
+      eapply eqb_term_spec. eauto.
+    - constructor.
   Qed.
   Next Obligation.
     destruct hΣ as [wΣ].
@@ -1877,15 +1953,12 @@ Section Conversion.
     eapply conv_alt_trans ; try eassumption.
     eapply conv_zipp.
     constructor.
-    eapply upto_names_impl_eq_term.
-    eapply elimT.
-    - eapply reflect_upto_names.
-    - symmetry. assumption.
+    eapply eqb_term_spec. eauto.
   Qed.
 
   (* tFix *)
   Next Obligation.
-    destruct hΣ as [wΣ].
+    (* destruct hΣ as [wΣ].
     eapply wellformed_alpha ; try assumption.
     - exact h2.
     - apply eq_term_upto_univ_sym ; auto.
@@ -1893,16 +1966,15 @@ Section Conversion.
       eapply elimT.
       + eapply reflect_upto_names.
       + symmetry. assumption.
-  Qed.
+  Qed. *)
+  Admitted.
   Next Obligation.
     unshelve eapply R_stateR.
     all: try reflexivity.
-    - simpl.
-      eapply ssrbool.elimT.
-      + eapply reflect_nleq_term.
-      + eapply nleq_term_zipc.
-        symmetry. assumption.
-    - simpl. constructor.
+    all: simpl.
+    - eapply eq_term_zipc.
+      eapply eqb_term_spec. eauto.
+    - constructor.
   Qed.
   Next Obligation.
     destruct hΣ as [wΣ].
@@ -1913,11 +1985,7 @@ Section Conversion.
     eapply conv_alt_trans ; try eassumption.
     eapply conv_zipp.
     constructor.
-    symmetry in eq1.
-    eapply upto_names_impl_eq_term.
-    eapply elimT.
-    - eapply reflect_upto_names.
-    - assumption.
+    eapply eqb_term_spec. eauto.
   Qed.
   Next Obligation.
     cbn. rewrite zipc_appstack. cbn.
@@ -2224,7 +2292,7 @@ Section Conversion.
 
   (* tCoFix *)
   Next Obligation.
-    destruct hΣ as [wΣ].
+    (* destruct hΣ as [wΣ].
     eapply wellformed_alpha ; try assumption.
     - exact h2.
     - apply eq_term_upto_univ_sym ; auto.
@@ -2232,16 +2300,15 @@ Section Conversion.
       eapply elimT.
       + eapply reflect_upto_names.
       + symmetry. assumption.
-  Qed.
+  Qed. *)
+  Admitted.
   Next Obligation.
     unshelve eapply R_stateR.
     all: try reflexivity.
-    - simpl.
-      eapply ssrbool.elimT.
-      + eapply reflect_nleq_term.
-      + eapply nleq_term_zipc.
-        symmetry. assumption.
-    - simpl. constructor.
+    all: simpl.
+    - eapply eq_term_zipc.
+      eapply eqb_term_spec. eauto.
+    - constructor.
   Qed.
   Next Obligation.
     destruct hΣ as [wΣ].
@@ -2251,11 +2318,7 @@ Section Conversion.
     eapply conv_alt_trans ; try eassumption.
     eapply conv_zipp.
     constructor.
-    symmetry in eq1.
-    eapply upto_names_impl_eq_term.
-    eapply elimT.
-    - eapply reflect_upto_names.
-    - assumption.
+    eapply eqb_term_spec. eauto.
   Qed.
 
   (* Fallback *)
@@ -2453,8 +2516,8 @@ Section Conversion.
     pose proof (decompose_stack_eq _ _ _ (eq_sym eq1)). subst.
     instantiate (1 := h2').
     simpl in H0. destruct H0 as [eq hp].
-    unshelve eapply R_positionR ; try assumption.
-    simpl. f_equal. assumption.
+    unshelve eapply R_positionR. 2: assumption.
+    simpl. rewrite eq. reflexivity.
   Qed.
   Next Obligation.
     pose proof (decompose_stack_eq _ _ _ (eq_sym eq1)). subst.
@@ -2747,132 +2810,6 @@ Section Conversion.
     - reflexivity.
   Qed.
 
-  Definition leqb_term :=
-    eqb_term_upto_univ (try_eqb_universe G) (try_leqb_universe G).
-
-  Definition eqb_term :=
-    eqb_term_upto_univ (try_eqb_universe G) (try_eqb_universe G).
-
-  Lemma leqb_term_spec t u :
-    leqb_term t u ->
-    leq_term (global_ext_constraints Σ) t u.
-  Proof.
-    pose proof hΣ'.
-    apply eqb_term_upto_univ_impl.
-    intros u1 u2; eapply (try_eqb_universe_spec G (global_ext_uctx Σ)); tas.
-    now eapply wf_ext_global_uctx_invariants.
-    now eapply global_ext_uctx_consistent.
-    intros u1 u2; eapply (try_leqb_universe_spec G (global_ext_uctx Σ)); tas.
-    now eapply wf_ext_global_uctx_invariants.
-    now eapply global_ext_uctx_consistent.
-  Qed.
-
-  Lemma eqb_term_spec t u :
-    eqb_term t u ->
-    eq_term (global_ext_constraints Σ) t u.
-  Proof.
-    pose proof hΣ'.
-    apply eqb_term_upto_univ_impl.
-    intros u1 u2; eapply (try_eqb_universe_spec G (global_ext_uctx Σ)); tas.
-    now eapply wf_ext_global_uctx_invariants.
-    now eapply global_ext_uctx_consistent.
-    intros u1 u2; eapply (try_eqb_universe_spec G (global_ext_uctx Σ)); tas.
-    now eapply wf_ext_global_uctx_invariants.
-    now eapply global_ext_uctx_consistent.
-  Qed.
-
-  Fixpoint eqb_ctx (Γ Δ : context) : bool :=
-    match Γ, Δ with
-    | [], [] => true
-    | {| decl_name := na1 ; decl_body := None ; decl_type := t1 |} :: Γ,
-      {| decl_name := na2 ; decl_body := None ; decl_type := t2 |} :: Δ =>
-      eqb_term t1 t2 && eqb_ctx Γ Δ
-    | {| decl_name := na1 ; decl_body := Some b1 ; decl_type := t1 |} :: Γ,
-      {| decl_name := na2 ; decl_body := Some b2 ; decl_type := t2 |} :: Δ =>
-      eqb_term b1 b2 && eqb_term t1 t2 && eqb_ctx Γ Δ
-    | _, _ => false
-    end.
-
-  Lemma eqb_ctx_spec :
-    forall Γ Δ,
-      eqb_ctx Γ Δ ->
-      eq_context_upto (eq_universe (global_ext_constraints Σ)) Γ Δ.
-  Proof.
-    intros Γ Δ h.
-    induction Γ as [| [na [b|] A] Γ ih ] in Δ, h |- *.
-    all: destruct Δ as [| [na' [b'|] A'] Δ].
-    all: try discriminate.
-    - constructor.
-    - simpl in h. apply andP in h as [h h3]. apply andP in h as [h1 h2].
-      constructor.
-      + eapply eqb_term_spec. assumption.
-      + eapply eqb_term_spec. assumption.
-      + eapply ih. assumption.
-    - simpl in h. apply andP in h as [h1 h2].
-      constructor.
-      + eapply eqb_term_spec. assumption.
-      + eapply ih. assumption.
-  Qed.
-
-  Definition eqb_term_stack t1 π1 t2 π2 :=
-    eqb_ctx (stack_context π1) (stack_context π2) &&
-    eqb_term (zipp t1 π1) (zipp t2 π2).
-
-  Lemma eqb_term_stack_spec :
-    forall Γ t1 π1 t2 π2,
-      eqb_term_stack t1 π1 t2 π2 ->
-      eq_context_upto (eq_universe (global_ext_constraints Σ))
-                      (Γ ,,, stack_context π1)
-                      (Γ ,,, stack_context π2) ×
-      eq_term (global_ext_constraints Σ) (zipp t1 π1) (zipp t2 π2).
-  Proof.
-    intros Γ t1 π1 t2 π2 h.
-    apply andP in h as [h1 h2].
-    split.
-    - eapply eq_context_upto_cat.
-      + eapply eq_context_upto_refl. intro. apply eq_universe_refl.
-      + eapply eqb_ctx_spec. assumption.
-    - eapply eqb_term_spec. assumption.
-  Qed.
-
-  Definition leqb_term_stack t1 π1 t2 π2 :=
-    eqb_ctx (stack_context π1) (stack_context π2) &&
-    leqb_term (zipp t1 π1) (zipp t2 π2).
-
-  Definition eqb_termp leq u v :=
-    match leq with
-    | Conv => eqb_term u v
-    | Cumul => leqb_term u v
-    end.
-
-  Lemma eqb_termp_spec :
-    forall leq u v Γ,
-      eqb_termp leq u v ->
-      conv leq Σ Γ u v.
-  Proof.
-    intros leq u v Γ e.
-    destruct leq.
-    - simpl. constructor. constructor. eapply eqb_term_spec. assumption.
-    - simpl. constructor. constructor. eapply leqb_term_spec. assumption.
-  Qed.
-
-  Lemma leqb_term_stack_spec :
-    forall Γ t1 π1 t2 π2,
-      leqb_term_stack t1 π1 t2 π2 ->
-      eq_context_upto (eq_universe (global_ext_constraints Σ))
-                      (Γ ,,, stack_context π1)
-                      (Γ ,,, stack_context π2) ×
-      leq_term (global_ext_constraints Σ) (zipp t1 π1) (zipp t2 π2).
-  Proof.
-    intros Γ t1 π1 t2 π2 h.
-    apply andP in h as [h1 h2].
-    split.
-    - eapply eq_context_upto_cat.
-      + eapply eq_context_upto_refl. intro. apply eq_universe_refl.
-      + eapply eqb_ctx_spec. assumption.
-    - eapply leqb_term_spec. assumption.
-  Qed.
-
   Equations(noeqns) _isconv_fallback (Γ : context) (leq : conv_pb)
             (t1 : term) (π1 : stack) (h1 : wtp Γ t1 π1)
             (t2 : term) (π2 : stack) (h2 : wtp Γ t2 π2)
@@ -2898,15 +2835,11 @@ Section Conversion.
           }
         } ;
       | @exist None _ with inspect leq := {
-        | @exist Conv eq1 with inspect (nleq_term t1 t2) := {
+        | @exist Conv eq1 with inspect (eqb_term t1 t2) := {
           | @exist true eq2 := isconv_args t1 π1 π2 aux ;
-          (* | @exist false _ := no *)
-          (* It should be useless, but as nleq_term might not see equal
-             universes, this might be a useful fallback.
-          *)
-          | @exist false _ := exist (eqb_term (zipp t1 π1) (zipp t2 π2)) _
+          | @exist false _ := no
           } ;
-        | @exist Cumul eq1 with inspect (nleq_term t1 t2) := {
+        | @exist Cumul eq1 with inspect (eqb_term t1 t2) := {
           | @exist true eq2 := isconv_args t1 π1 π2 aux ;
           | @exist false _ := exist (leqb_term (zipp t1 π1) (zipp t2 π2)) _
           }
@@ -3213,7 +3146,7 @@ Section Conversion.
     - eapply conv_context_sym. all: auto.
   Qed.
   Next Obligation.
-    destruct hΣ as [wΣ].
+    (* destruct hΣ as [wΣ].
     eapply wellformed_alpha ; try assumption.
     - exact h2.
     - apply eq_term_upto_univ_sym ; auto.
@@ -3221,13 +3154,12 @@ Section Conversion.
       eapply elimT.
       + eapply reflect_upto_names.
       + symmetry. assumption.
-  Qed.
+  Qed. *)
+  Admitted.
   Next Obligation.
     eapply R_stateR. all: simpl. all: try reflexivity.
-    - eapply ssrbool.elimT.
-      + eapply reflect_nleq_term.
-      + eapply nleq_term_zipc.
-        symmetry. assumption.
+    - eapply eq_term_zipc.
+      eapply eqb_term_spec. eauto.
     - constructor.
   Qed.
   Next Obligation.
@@ -3240,19 +3172,17 @@ Section Conversion.
     - eassumption.
     - eapply conv_zipp.
       constructor.
-      eapply upto_names_impl_eq_term.
-      eapply elimT.
-      + eapply reflect_upto_names.
-      + eauto.
+      eapply eqb_term_spec. eauto.
   Qed.
   Next Obligation.
-    case_eq (eqb_term (zipp t1 π1) (zipp t2 π2)). 2: auto.
+    (* case_eq (eqb_term (zipp t1 π1) (zipp t2 π2)). 2: auto.
     intro e.
     apply eqb_term_spec in e.
     constructor. constructor. assumption.
-  Qed.
+  Qed. *)
+  Admitted.
   Next Obligation.
-    destruct hΣ as [wΣ].
+    (* destruct hΣ as [wΣ].
     eapply wellformed_alpha ; try assumption.
     - exact h2.
     - apply eq_term_upto_univ_sym ; auto.
@@ -3260,15 +3190,14 @@ Section Conversion.
       eapply elimT.
       + eapply reflect_upto_names.
       + symmetry. assumption.
-  Qed.
-  Next Obligation.
+  Qed. *)
+  Admitted.
+  (* Next Obligation.
     eapply R_stateR. all: simpl. all: try reflexivity.
-    - eapply ssrbool.elimT.
-      + eapply reflect_nleq_term.
-      + eapply nleq_term_zipc.
-        symmetry. assumption.
+    - eapply eq_term_zipc.
+      eapply eqb_term_spec. eauto.
     - constructor.
-  Qed.
+  Qed. *)
   Next Obligation.
     destruct b. 2: auto.
     destruct h as [h].
@@ -3279,10 +3208,8 @@ Section Conversion.
     - eapply conv_alt_cumul. all: eauto.
     - eapply cumul_zipp.
       constructor.
-      eapply upto_names_impl_leq_term.
-      eapply elimT.
-      + eapply reflect_upto_names.
-      + eauto.
+      eapply eq_term_leq_term.
+      eapply eqb_term_spec. eauto.
   Qed.
   Next Obligation.
     case_eq (leqb_term (zipp t1 π1) (zipp t2 π2)). 2: auto.
